
\begin{equation*}
	C = A B =  f(A, B)
\end{equation*}

\begin{equation*}
	C = f(A + A', B) = f(A, B) + f(A', B)
\end{equation*}

\begin{align*}
	c_1 &= t_{111} a_1 b_1 + t_{112} a_1 b_2 + t_{121} a_2 b_1 + t_{122} a_2 b_2 \\
	c_2 &= t_{211} a_1 b_1 + t_{212} a_1 b_2 + t_{221} a_2 b_1 + t_{222} a_2 b_2 
\end{align*}

\begin{equation*}
	C_i = \sum_{jk} T_{ijk} A_j B_k
\end{equation*}

\begin{equation*}
	C_i = T_{ijk} A_j B_k
\end{equation*}

\begin{equation*}
	M_{ij} = \sum_{\lambda = 1}^r u^\lambda_i v^\lambda_j
\end{equation*}

\begin{equation*}
	\begin{pmatrix}
	    2 & 1 \\
	    1 & 0 \\
	\end{pmatrix}
	= 
	\begin{pmatrix}1 \\ 0\end{pmatrix}\begin{pmatrix}1 & 1\end{pmatrix}
	+
	\begin{pmatrix}1 \\ 1\end{pmatrix}\begin{pmatrix}1 & 0\end{pmatrix}
\end{equation*}


\begin{equation*}
	T_{ijk} = \sum_{\lambda = 1}^r u^\lambda_i v^\lambda_j w^\lambda_k
\end{equation*}

\begin{equation*}
	C_i = \sum_{\lambda=1}^r u_i^\lambda (v_j^\lambda A_j) (w_k^\lambda B_k)
\end{equation*}