Consider 1D non-interacting electrons described by the Hamiltonian
\begin{equation*}
	\hat{H} = \sum_k \xi_k \hat{c}_k\D \hat{c}_k,
	\hspace{10 mm} 
	\xi_k = \varepsilon_k - \mu.
\end{equation*}
We want to compute the Linchard function $\chi_0$
is the
correlation function
associated
with the
response
to
a
change
of the
chemical
potential.


\textbf{1. Lindhard function}.  The density response function $\chi_0(q, \omega)$ of a one-dimensional Fermi gas 
\begin{equation*}
	\chi_0(q, t) = - \frac{i}{\hbar} \theta(t) \langle [\hat{\rho}_q(t), \hat{\rho}_{-q} (0)]\rangle,
\end{equation*}
% with thermal expectation value over $\rho = e^{- \beta H} / Z$. Here 
% \begin{equation*}
% 	\hat{\rho}_q \overset{\mathrm{n}}{=}  \sum_k \hat{c}_{k+q}\D \hat{c}_k,
% \end{equation*}
% is the Fourier transform of the density operator $\hat{\rho}_r = \hat{\psi}\D(r) \hat{\psi}(r)$
% \begin{equation*}
% 	\hat{\rho}_q \overset{\mathrm{n}}{=} \int dr \ \hat{\psi}\D(r) \hat{\psi}(r)  e^{- i q r}.
% \end{equation*}
% The time evolution $\hat{\rho}_q$  is given by
% \begin{equation*}
% 	\hat{\rho}_q (t) \overset{\mathrm{n}}{=} \sum_k e^{i (\xi_{k+q}-\xi_k)t} \hat{c}_{k+q}\D \hat{c}_k. 
% \end{equation*}
Thus we find for the Fourier transform of the Lindhard function	
\begin{equation*}
	\chi_0 (q, \omega) = - \frac{i}{\hbar} \int_{-\infty}^{\infty} dt \ 
	e^{i \omega t} \theta(t) \langle [\hat{\rho}_q(t), \hat{\rho}_{-q} (0)]\rangle = - \frac{i}{\hbar V} \sum_k \int_{0}^{\infty} dt\ 
	e^{i(\omega - (\xi_k - \xi_{k+q}))t} \left[
		n_{k+q} (1-n_k) - n_k (1 - n_{k+q})
	\right],
\end{equation*}
where we took advantage of the quadratic Hamiltonian of free fermions. 
\begin{equation*}
	\chi_0 (q, \omega) = \frac{1}{\hbar V} \sum_k \frac{n_{k+q} - n_k}{\omega- (\xi_k - \xi_{k+q}) + 0 i}.
\end{equation*}
% \red{
% If we use other defininiton $\hat{\rho}_q = \sum_k \hat{c}_k \hat{c}_{k+q}$, then
% \begin{equation*}
% 	\chi_0 (q, \theta) = \frac{1}{\hbar V} \sum_k \frac{n_{k+q}- n_k}{\omega + (\xi_k - \xi_{j+q}) + 0i}.
% \end{equation*}
% Using that
% \begin{equation*}
% 	\lim_{\eta \to 0} \frac{1}{\omega + i \eta} = \mathcal{P}\left(\frac{1}{\omega}\right) - i \pi \delta(\omega).
% \end{equation*}
% }
Moving on to integration
\begin{equation*}
	\chi_0 (q,\omega) = \frac{1}{V \hbar} \int_{-\infty}^{\infty} \frac{dk}{2\pi} \frac{n_{k+q} - n_k}{\omega- (\xi_k - \xi_{k+q}) + 0 i} = \mathcal{P} \int_{-\infty}^{\infty} \frac{dk}{2\pi} \frac{n_{k+q} - n_k}{\omega- (\xi_k - \xi_{k+q})} - i \pi \int_{-\infty}^{\infty} \frac{dk}{2\pi} 
	\left(n_{k+q} - n_k\right) \delta(\omega - (\xi_{k+q}-\xi_k)),
\end{equation*}
we get
\begin{align*}
	\chi_0''(q,\omega) &= \Im \chi_0 (q, \omega) = \frac{1}{2} \int_{-\infty}^{\infty} dk\ \left(
		\delta(\omega - (\xi_{k+q}-\xi_k)) - \delta(\omega - (\xi_k - \xi_{k-1}))
	\right) n_k 
	\\ &= 
	\frac{m}{2|q|} \int_{-\infty}^{\infty} n_k (\delta(k-k_-) - \delta(k - k_+)) \d k = \frac{m}{2|q|} \left(
		n_{k_-} - n_{k_+}
	\right)
	,
\end{align*}
with defined zeros 
\begin{equation*}
	\delta(\omega - (\xi_{k+q} - \xi_k)) = \frac{m}{|q|} \delta(k - k_\pm),
	\hspace{10 mm} 
	k_{\pm} = \frac{2 m \omega \pm q^2}{2q}.
\end{equation*}
