Writing the path as $q(t) = q_c(t) = y(t)$, due to $\delta S[q_c(t)] = 0$ we could rewrite $S$ as 
\begin{equation*}
	S[q(t)] = \int_{0}^{T} \frac{m}{2}\left(
		(\dot{q}_c + \dot{y})^2 - \omega^2 (q_c + y)^2
	\right) \d t = S[q_c(t)] + S[y(t)] + \int_{0}^{T} m\left(
		\dot{q}_c \d y - \omega^2 q_c y \d t
	\right)  = S[q_c(t)] + S[y(t)].
\end{equation*}
It was used that Euler-Lagrange equation $\partial_x L - \frac{d }{d t} \partial_{\dot{x}} L = 0$ leads to classical equation of motion $\ddot{q}_c = - m \omega^2 q_c(t)$:
\begin{equation*}
	\int_{0}^{T}  m \dot{q}_c \d y = y(t) \dot{q}_c \bigg|_0^T - \int_{0}^{T} m y \ddot{q}_c \d t = \int_{0}^{T}  m \omega^2 y q_c \d t. 
\end{equation*}
Thus we could factorise $K$
\begin{equation*}
	K = e^{i S[q_c(t)]} F(T),
	\hspace{10 mm} 
	F(T) = \int e^{i S[y(t)]} \F y(t).
\end{equation*}
