Consider the Hamiltonian
\begin{equation*}
  \hat{H} = \omega\left(\hat{a}\D \hat{a} + \tfrac{1}{2}\right) + \tfrac{1}{2} \omega_0 \hat{\sigma}_z + \chi \hat{\sigma}_z \left(
    \hat{a}\D \hat{a} + \tfrac{1}{2}
  \right),
\end{equation*}
with $\chi = g^2 / \Delta$. Eigenavalues could be expressed as \textbf{(a)}
\begin{equation*}
  E_n^g = \omega (n + \tfrac{1}{2}) - \frac{\omega_0}{2} -\chi (n + \tfrac{1}{2}),
  \hspace{5 mm} 
     E_n^e = \omega (n + \tfrac{1}{2}) + \frac{\omega_0}{2} +\chi (n + \tfrac{1}{2})
\end{equation*}
corresponding eigenstates $\ket{g, n}$ and $\ket{e, n}$.

Evoultion is just \textbf{(b)}
\begin{align*}
  \hat{U}(t_0) (\ket{g,0} + \ket{e,0}) &= \ket{g,0} - i e^{-i \omega_0 t_0} \ket{e,0}, \\
  \hat{U}(t_0) (\ket{g,1} + \ket{e,1}) &= \ket{g,0} + i e^{-i \omega_0 t_0} \ket{e,0},
\end{align*}
with $t_0 = \tfrac{\pi}{2} / \chi$.  For coherent state  \textbf{(c)}
\begin{equation*}
  \hat{U}(t_0) \ket{g,0}  = e^{-\frac{|\alpha|^2}{2}} \sum_{n=0}^{\infty} e^{-i E_n^g t} \frac{\alpha^n \ket{g, n}}{\sqrt{n!}},
  \hspace{10 mm} 
  \hat{U}(t_0) \ket{e,0}  = e^{-\frac{|\alpha|^2}{2}} \sum_{n=0}^{\infty} e^{-i E_n^e t} \frac{\alpha^n \ket{e, n}}{\sqrt{n!}}.
\end{equation*}
