% f


% 
% 
% 



\begin{equation*}
	\sum_a v_a' = \sum_a \sum_b P_{ab} v_b = \sum_b v_b \sum_a P_{ab} = \sum_b v_b = 1 + \overset{1}{2}
\end{equation*}

Consider the system with Hamiltonian
\begin{equation*}
	\hat{H} = - \frac{\omega_0}{2} \hat{\sigma}_z + \omega_1 \cos(\omega t) \hat{\sigma}_x
\end{equation*}


\begin{align*}
	e^{-i\omega t/2} \alpha(t) &= \cos\left(\frac{\Omega t}{2}\right) - i \frac{\Delta}{\Omega} \sin\left(\frac{\Omega t}{2}\right), \\
	e^{i\omega t/2} \beta(t) &= -i \frac{\omega_1}{\Omega} \sin\left(\frac{\Omega t}{2}\right),
\end{align*}

\begin{equation*}
	\ket{\psi} = \alpha(t) \ket{0} + \beta(t) \ket{1}
\end{equation*}

$$ e^{i\omega t/2} \beta (t) = -i \frac{\omega_1}{\Omega} \sin\left(\frac{\Omega t}{2}\right)$$