\subsection{Quantum State Tomography}

\begin{enumerate}[label=(\alph*)]
	\item \input{parts/hw21_a}
	\item \input{parts/hw21_b}
\end{enumerate}


\subsection{Semi-Classical Lightâ€“Matter Interaction}

We have basic light-atom interaction
\begin{equation*}
	\hat{H} = \hat{H}_0 + \hat{V}
	,
	\hspace{10 mm} 
	\hat{H}_0 = - \frac{\hbar \omega}{2} \hat{\sigma}_z,
	\hspace{5 mm} 
	\hat{V}(t) = - \hbar \Omega \cos(\omega_L t) \hat{\sigma}_x,
\end{equation*}
with Rabi frequency $\Omega = d E_0 / \hbar$.

\begin{enumerate}[label=(\alph*)]
	\item \input{parts/hw22_a}
	\item \input{parts/hw22_b}
	\item \input{parts/hw22_c}
	\item \input{parts/hw22_d}
	\item \input{parts/hw22_e}
	\item \input{parts/hw22_f}
	\item \input{parts/hw22_g}
\end{enumerate}



\subsection{Driven System Dynamics and Rotating-Wave Approximation}

Consider $H_0 = - \frac{\hbar \omega}{2} \sigma_z$ with $V = \frac{\hbar\Omega}{2}\cos(\omega t) \sigma_z - \frac{\hbar\Omega}{2} \sin(\omega t) \sigma_y $ (black dashed line) and $\sub{V}{RWA} = \hbar \Omega \cos(\omega t) \sigma_x$ (\blue{blue} line) in resonant $(\omega=\omega_0)$ case (fig. \ref{fig:rwa}).

\begin{figure}[h]
    \centering
    \includegraphics[width=1.0\textwidth]{figs/p23_1.pdf}
    \caption{Comparison of the exact solution (black) and the solution in the rotating wave approximation (blue).}
    \label{fig:rwa}
\end{figure}


We could find solution in general case $\delta \neq 0$ in RWA:
\begin{equation*}
	\langle \sigma_z\rangle(t) = \cos (\Omega_\delta t) + \frac{\delta ^2}{\delta ^2+\Omega ^2}(1-\cos (\Omega_\delta t )),
	\hspace{10 mm} 
	\Omega_\delta = \sqrt{\Omega^2 + \delta^2},
\end{equation*}
with general Rabi frequency $\Omega_\delta$. For different $\delta = 0, \Omega, 2 \Omega$ and $\Omega=2\pi$ we could compare different behaviour (fig. \ref{fig:rod}).

\begin{figure}[h]
    \centering
    \includegraphics[width=0.75\textwidth]{figs/p23_2.pdf}
    \caption{Rabi oscillations at different detuning values}
    \label{fig:rod}
\end{figure}


\subsection{Dephasing and Decoherence in a TLS}

We could calculate $\langle \vc{\sigma}\rangle$, using  \eqref{leq}:
\begin{equation*}
	\rho(t) = \begin{pmatrix}
	    1-|\beta|^2 e^{- \Gamma_1 t} & \alpha \bar{\beta} e^{-\Gamma_2 t} \\
	    \bar{\alpha} \beta e^{- \Gamma_2 t} & |\beta|^2 e^{-\Gamma_1 t} \\
	\end{pmatrix},
	\hspace{0.5cm} \Rightarrow \hspace{0.5cm}
	\left.\begin{aligned}
	   \langle \sigma_x\rangle &= (\alpha \bar{\beta} + \bar{\alpha} \beta ) e^{- \Gamma_2 t}\\
	   \langle \sigma_y\rangle &= i(\alpha \bar{\beta} - \bar{\alpha} \beta ) e^{- \Gamma_2 t} \\
	   \langle \sigma_z\rangle &= 1 - 2 |\beta|^2 e^{-t \Gamma_1}
	\end{aligned}\right.
\end{equation*}
Substituting the initial state $\tfrac{1}{\sqrt{2}}\ket{0} + \tfrac{1}{\sqrt{2}}\ket{1}$
\begin{equation*}
	\langle \sigma_x\rangle =  e^{- \Gamma_2 t},
	\hspace{10 mm} 
	\langle \sigma_y\rangle = 0,
	\hspace{10 mm}
	\langle \sigma_z\rangle = 1 - e^{- \Gamma_1 t},
\end{equation*}
thus by measuring the various components we can find the $\Gamma_1$ and $\Gamma_2$, it's just exponential decay.


